code/InsertWorksProofs.v
@@ -854,12 +854,7 @@ Proof.
           apply cut_right_not_nil; simpl; try assumption; try omega.
 Qed.
 
-Theorem appears_kvl_appears_leaf_tree: forall {X: Type} (b: nat) k l,
-  appears_in_kvl k l -> appears_in_tree k (bptLeaf b X l).
-Proof.
-  intros. induction H. apply ait_leaf. apply ai_here. apply ait_leaf.
-  eapply appears_in_super_set_appears. reflexivity. apply H.
-Qed.
+
 
 
 Lemma insert_not_split_impl_space_left: forall {X: Type} (b: nat) k (v:X) l l',
@@ -878,62 +873,7 @@ Proof.
 Qed.
 
 
-Lemma appears_in_split_node_appears_in_lists: forall {X: Type} b k n left right, 
-  kvl_sorted (left ++ right) ->
-  key_at_index 0 right = Some n ->
-  appears_in_kvl k left \/ appears_in_kvl k right ->
-  appears_in_tree k (bptNode b X [(0, bptLeaf b X left), (n, bptLeaf b X right)]).
-Proof.
-  intros. destruct H1. 
-  Case "Left hand side".
-    apply ait_node_here. apply ait_leaf. assumption. destruct right.
-    simpl in H0. inversion H0. inversion H0. destruct p. inversion H3. subst.
-    apply appears_in_kvl_app in H1. do 3 destruct H1. subst. 
-    rewrite <- app_assoc in H. apply kvl_sorted_app with (l1:=witness) in H. destruct H.
-    apply kvl_sorted_key_across_app in H1. omega.
-  Case "Right hand side".
-    apply ait_node_later. apply ait_node_one. apply ait_leaf. assumption. 
-    SCase "n <=".
-      inversion H0. destruct right. inversion H3. destruct p. inversion H3. subst. remember (beq_nat n k).
-      destruct b0. symmetry in Heqb0. apply beq_nat_true in Heqb0. subst. omega.
-      apply appears_cons in H1. apply appears_in_kvl_app in H1. do 3 destruct H1. subst.
-      apply kvl_sorted_app with (l1:=left) in H. inversion H. 
-      apply kvl_sorted_key_across_app in H2.  omega. symmetry in Heqb0. 
-      apply beq_nat_false in Heqb0. omega.
-    SCase "< n".
-    inversion H0. destruct right. inversion H3. destruct p. inversion H3. subst.
-    remember (beq_nat n k).
-    destruct b0. symmetry in Heqb0. apply beq_nat_true in Heqb0. subst. omega.
-    apply appears_cons in H1. apply appears_in_kvl_app in H1. do 3 destruct H1. subst.
-    apply kvl_sorted_app with (l1:=left) in H. inversion H. 
-    apply kvl_sorted_key_across_app in H2. omega. symmetry in Heqb0. 
-    apply beq_nat_false in Heqb0. omega.
-Qed.
 
-
-Lemma key_at_index_0none_impl_empty: forall (X: Type) l,
-  @key_at_index X 0 l = None -> l = [].
-Proof. 
-  intros. unfold key_at_index in H. destruct l. reflexivity. destruct p. inversion H.
-Qed.
-
-Lemma insert_leaf_preserves_sort: forall (X: Type) b k (v:X) l l1 l2,
-  kvl_sorted l ->
-  insert_leaf b k v l = (l1, Some l2) ->
-  kvl_sorted(l1 ++ l2).
-Proof.
-  intros.
-  unfold insert_leaf in H0.
-  remember (ble_nat (length (insert_into_list k v l)) (b * 2)).
-  destruct b0.
-  inversion H0.
-  remember (split_list b (insert_into_list k v l)). destruct p.
-  symmetry in Heqp. apply split_list_preserves_lists in Heqp.
-  inversion H0. subst.
-  assert (kvl_sorted (insert_into_list k v l)).
-    apply insert_preserves_sort. apply H.
-  rewrite Heqp in H1. apply H1.
-Qed.
 
 Theorem insert_works : forall {X: Type} {b: nat} (t t1: bplustree b X) (k: nat) (v: X),
   valid_bplustree b X t -> 
