code/SortingProofs.v
@@ -212,6 +212,24 @@ Proof.
       subst. apply blt_nat_true in H7. omega.
 Qed.
 
+Lemma insert_leaf_preserves_sort: forall (X: Type) b k (v:X) l l1 l2,
+  kvl_sorted l ->
+  insert_leaf b k v l = (l1, Some l2) ->
+  kvl_sorted(l1 ++ l2).
+Proof.
+  intros.
+  unfold insert_leaf in H0.
+  remember (ble_nat (length (insert_into_list k v l)) (b * 2)).
+  destruct b0.
+  inversion H0.
+  remember (split_list b (insert_into_list k v l)). destruct p.
+  symmetry in Heqp. apply split_list_preserves_lists in Heqp.
+  inversion H0. subst.
+  assert (kvl_sorted (insert_into_list k v l)).
+    apply insert_preserves_sort. apply H.
+  rewrite Heqp in H1. apply H1.
+Qed.
+
 Lemma split_preserves_sort : forall (X: Type) (l l1 l2: list (nat * X)),
   l1 ++ l2 = l -> kvl_sorted l -> kvl_sorted l1 /\ kvl_sorted l2.
 Proof.
